backend/LTL.v
@@ -135,7 +135,7 @@ Inductive state : Type :=
       state
   | Callstate:
       forall (stack: list stackframe) (**r call stack *)
-             (f: fundef)              (**r function to call *)
+             (fb: block)              (**r function to call *)
              (ls: locset)             (**r location state of caller *)
              (m: mem),                (**r memory state *)
       state
@@ -165,14 +165,13 @@ Definition destroyed_by_getstack (s: slot): list mreg :=
   | _        => nil
   end.
 
-Definition find_function (ros: mreg + ident) (rs: locset) : option fundef :=
+Definition find_block (ros: mreg + ident) (rs: locset) : option block :=
   match ros with
-  | inl r => Genv.find_funct ge (rs (R r))
-  | inr symb =>
-      match Genv.find_symbol ge symb with
-      | None => None
-      | Some b => Genv.find_funct_ptr ge b
-      end
+  | inl r => match rs (R r) with
+            | Vptr b o => Some b
+            | _ => None
+            end
+  | inr symb => Genv.find_symbol ge symb
   end.
 
 (** [parent_locset cs] returns the mapping of values for locations
@@ -214,18 +213,20 @@ Inductive step: state -> trace -> state -> Prop :=
       rs' = undef_regs (destroyed_by_store chunk addr) rs ->
       step (Block s f sp (Lstore chunk addr args src :: bb) rs m)
         E0 (Block s f sp bb rs' m')
-  | exec_Lcall: forall s f sp sig ros bb rs m fd,
-      find_function ros rs = Some fd ->
+  | exec_Lcall: forall s f sp sig ros bb rs m fb fd,
+      find_block ros rs = Some fb ->
+      Genv.find_funct_ptr ge fb = Some fd ->
       funsig fd = sig ->
       step (Block s f sp (Lcall sig ros :: bb) rs m)
-        E0 (Callstate (Stackframe f sp rs bb :: s) fd rs m)
-  | exec_Ltailcall: forall s f sp sig ros bb rs m fd rs' m',
+        E0 (Callstate (Stackframe f sp rs bb :: s) fb rs m)
+  | exec_Ltailcall: forall s f sp sig ros bb rs m fb fd rs' m',
       rs' = return_regs (parent_locset s) rs ->
-      find_function ros rs' = Some fd ->
+      find_block ros rs' = Some fb ->
+      Genv.find_funct_ptr ge fb = Some fd ->
       funsig fd = sig ->
       Mem.free m sp 0 f.(fn_stacksize) = Some m' ->
       step (Block s f (Vptr sp Ptrofs.zero) (Ltailcall sig ros :: bb) rs m)
-        E0 (Callstate s fd rs' m')
+        E0 (Callstate s fb rs' m')
   | exec_Lbuiltin: forall s f sp ef args res bb rs m vargs t vres rs' m',
       eval_builtin_args ge rs sp m args vargs ->
       external_call ef ge vargs m t vres m' ->
@@ -251,16 +252,18 @@ Inductive step: state -> trace -> state -> Prop :=
       Mem.free m sp 0 f.(fn_stacksize) = Some m' ->
       step (Block s f (Vptr sp Ptrofs.zero) (Lreturn :: bb) rs m)
         E0 (Returnstate s (return_regs (parent_locset s) rs) m')
-  | exec_function_internal: forall s f rs m m' sp rs',
+  | exec_function_internal: forall s fb f rs m m' sp rs',
+      Genv.find_funct_ptr ge fb = Some (Internal f) ->
       Mem.alloc m 0 f.(fn_stacksize) = (m', sp) ->
       rs' = undef_regs destroyed_at_function_entry (call_regs rs) ->
-      step (Callstate s (Internal f) rs m)
+      step (Callstate s fb rs m)
         E0 (State s f (Vptr sp Ptrofs.zero) f.(fn_entrypoint) rs' m')
-  | exec_function_external: forall s ef t args res rs m rs' m',
+  | exec_function_external: forall s fb ef t args res rs m rs' m',
+      Genv.find_funct_ptr ge fb = Some (External ef) ->
       args = map (fun p => Locmap.getpair p rs) (loc_arguments (ef_sig ef)) ->
       external_call ef ge args m t res m' ->
       rs' = Locmap.setpair (loc_result (ef_sig ef)) res rs ->
-      step (Callstate s (External ef) rs m)
+      step (Callstate s fb rs m)
          t (Returnstate s rs' m')
   | exec_return: forall f sp rs1 bb s rs m,
       step (Returnstate (Stackframe f sp rs1 bb :: s) rs m)
@@ -280,7 +283,7 @@ Inductive initial_state (p: program): state -> Prop :=
       Genv.find_symbol ge p.(prog_main) = Some b ->
       Genv.find_funct_ptr ge b = Some f ->
       funsig f = signature_main ->
-      initial_state p (Callstate nil f (Locmap.init Vundef) m0).
+      initial_state p (Callstate nil b (Locmap.init Vundef) m0).
 
 Inductive final_state: state -> int -> Prop :=
   | final_state_intro: forall rs m retcode,
