backend/RTLtyping.v
@@ -882,25 +882,6 @@ Inductive wt_stackframes: list stackframe -> signature -> Prop :=
       wt_stackframes s (fn_sig f) ->
       wt_stackframes (Stackframe res f sp pc rs :: s) sg.
 
-Inductive wt_state: state -> Prop :=
-  | wt_state_intro:
-      forall s f sp pc rs m env
-        (WT_STK: wt_stackframes s (fn_sig f))
-        (WT_FN: wt_function f env)
-        (WT_RS: wt_regset env rs),
-      wt_state (State s f sp pc rs m)
-  | wt_state_call:
-      forall s f args m,
-      wt_stackframes s (funsig f) ->
-      wt_fundef f ->
-      Val.has_type_list args (sig_args (funsig f)) ->
-      wt_state (Callstate s f args m)
-  | wt_state_return:
-      forall s v m sg,
-      wt_stackframes s sg ->
-      Val.has_type v (proj_sig_res sg) ->
-      wt_state (Returnstate s v m).
-
 Remark wt_stackframes_change_sig:
   forall s sg1 sg2,
   sg1.(sig_res) = sg2.(sig_res) -> wt_stackframes s sg1 -> wt_stackframes s sg2.
@@ -909,6 +890,34 @@ Proof.
 - constructor; congruence.
 - econstructor; eauto. rewrite H3. unfold proj_sig_res. rewrite H. auto.
 Qed.
+
+Section WTSTATE.
+
+  Variable p: program.
+
+  Let ge := Genv.globalenv p.
+
+  Inductive wt_state: state -> Prop :=
+  | wt_state_intro:
+      forall s f sp pc rs m env
+        (WT_STK: wt_stackframes s (fn_sig f))
+        (WT_FN: wt_function f env)
+        (WT_RS: wt_regset env rs),
+        wt_state (State s f sp pc rs m)
+  | wt_state_call:
+      forall s fb f args m,
+        Genv.find_funct_ptr ge fb = Some f ->
+        wt_stackframes s (funsig f) ->
+        wt_fundef f ->
+        Val.has_type_list args (sig_args (funsig f)) ->
+        wt_state (Callstate s fb args m)
+  | wt_state_return:
+      forall s v m sg,
+        wt_stackframes s sg ->
+        Val.has_type v (proj_sig_res sg) ->
+        wt_state (Returnstate s v m).
+
+End WTSTATE.
 
 Section SUBJECT_REDUCTION.
 
@@ -920,7 +929,7 @@ Let ge := Genv.globalenv p.
 
 Lemma subject_reduction:
   forall st1 t st2, step ge st1 t st2 ->
-  forall (WT: wt_state st1), wt_state st2.
+  forall (WT: wt_state p st1), wt_state p st2.
 Proof.
   induction 1; intros; inv WT;
   try (generalize (wt_instrs _ _ WT_FN pc _ H); intros WTI).
@@ -934,28 +943,18 @@ Proof.
   econstructor; eauto.
   (* Icall *)
   assert (wt_fundef fd).
-    destruct ros; simpl in H0.
-    pattern fd. apply Genv.find_funct_prop with fundef unit p (rs#r).
-    exact wt_p. exact H0.
-    caseEq (Genv.find_symbol ge i); intros; rewrite H1 in H0.
-    pattern fd. apply Genv.find_funct_ptr_prop with fundef unit p b.
-    exact wt_p. exact H0.
-    discriminate.
+    apply Genv.find_funct_ptr_prop with fundef unit p fb.
+    exact wt_p. exact H1.
   econstructor; eauto.
   econstructor; eauto. inv WTI; auto.
-  inv WTI. rewrite <- H8. apply wt_regset_list. auto.
+  inv WTI. rewrite <- H9. apply wt_regset_list. auto.
   (* Itailcall *)
   assert (wt_fundef fd).
-    destruct ros; simpl in H0.
-    pattern fd. apply Genv.find_funct_prop with fundef unit p (rs#r).
-    exact wt_p. exact H0.
-    caseEq (Genv.find_symbol ge i); intros; rewrite H1 in H0.
-    pattern fd. apply Genv.find_funct_ptr_prop with fundef unit p b.
-    exact wt_p. exact H0.
-    discriminate.
+    pattern fd. apply Genv.find_funct_ptr_prop with fundef unit p fb.
+    exact wt_p. exact H1.
   econstructor; eauto.
   inv WTI. apply wt_stackframes_change_sig with (fn_sig f); auto.
-  inv WTI. rewrite <- H7. apply wt_regset_list. auto.
+  inv WTI. rewrite <- H8. apply wt_regset_list. auto.
   (* Ibuiltin *)
   econstructor; eauto. eapply wt_exec_Ibuiltin; eauto.
   (* Icond *)
@@ -966,10 +965,12 @@ Proof.
   econstructor; eauto.
   inv WTI; simpl. auto. unfold proj_sig_res; rewrite H2. auto.
   (* internal function *)
-  simpl in *. inv H5.
+  assert (f0 = Internal f) by (unfold ge in *; congruence). subst.
+  simpl in *. inv H7.
   econstructor; eauto.
-  inv H1. apply wt_init_regs; auto. rewrite wt_params0. auto.
+  inv H2. apply wt_init_regs; auto. rewrite wt_params0. auto.
   (* external function *)
+  assert (f = External ef) by (unfold ge in *; congruence). subst.
   econstructor; eauto. simpl.
   eapply external_call_well_typed; eauto.
   (* return *)
@@ -978,9 +979,9 @@ Proof.
 Qed.
 
 Lemma wt_initial_state:
-  forall S, initial_state p S -> wt_state S.
+  forall S, initial_state p S -> wt_state p S.
 Proof.
-  intros. inv H. constructor. constructor. rewrite H3; auto.
+  intros. inv H. econstructor. unfold ge0 in *; eauto. constructor. rewrite H3; auto.
   pattern f. apply Genv.find_funct_ptr_prop with fundef unit p b.
   exact wt_p. exact H2.
   rewrite H3. constructor.
@@ -988,7 +989,7 @@ Qed.
 
 Lemma wt_instr_inv:
   forall s f sp pc rs m i,
-  wt_state (State s f sp pc rs m) ->
+  wt_state p (State s f sp pc rs m) ->
   f.(fn_code)!pc = Some i ->
   exists env, wt_instr f env i /\ wt_regset env rs.
 Proof.
